doc: fill paragraphs

Notes/Anselm.lean
@@ -9,92 +9,74 @@ import Mathlib.Order.Bounds.Basic
 /-!
 # St. Anselm's ontological argument
 
-The [`Anselm`][anselm] file might be the second attempt in the Lean
-community to formalize an ontological argument for the existence of God
-in Lean. It's a modified version of the formulation of St. Anselm's
-ontological argument by Alvin Plantinga. (See [9.1 Formulation
-1][plantinga] of the SEP entry ["Ontological Arguments."](#reference))
+The [`Anselm`][anselm] file might be the second attempt in the Lean community to formalize an
+ontological argument for the existence of God in Lean. It's a modified version of the formulation of
+St. Anselm's ontological argument by Alvin Plantinga. (See [9.1 Formulation 1][plantinga] of the SEP
+entry ["Ontological Arguments."](#reference))
 
-1. God exists in the understanding but not in reality. (Assumption for
-   *reductio*)
-2. Existence in reality is greater than existence in the understanding
-   alone. (Premise)
-3. There exists a being in reality that can be conceived. (*Modified*
-   premise)
-4. A being that exists in reality and can be conceived is greater than
-   God. (From (1) and (2).)
-5. There exists a being that can be conceived and is greater than God.
-   (From (3) and (4).)
-6. No being greater than God can be conceived. (From the definition of
-   “God”.)
-7. Hence, it is false that God exists in the understanding but not in
-   reality. (From (1), (5), (6).)
-8. God exists in the understanding. (Premise, to which even the Fool
-   agrees.)
+1. God exists in the understanding but not in reality. (Assumption for *reductio*)
+2. Existence in reality is greater than existence in the understanding alone. (Premise)
+3. There exists a being in reality that can be conceived. (*Modified* premise)
+4. A being that exists in reality and can be conceived is greater than God. (From (1) and (2).)
+5. There exists a being that can be conceived and is greater than God.  (From (3) and (4).)
+6. No being greater than God can be conceived. (From the definition of “God”.)
+7. Hence, it is false that God exists in the understanding but not in reality. (From (1), (5), (6).)
+8. God exists in the understanding. (Premise, to which even the Fool agrees.)
 9. Hence God exists in reality. (From (7), (8).)
 
 I formalized the three premises of the argument as follows:
 
-* `lt_of_inUnderstanding_not_inReality_inReality {x y : Being} :
-InUnderstanding x → ¬InReality x → InReality y → x < y` (Step 2)
-* `exists_conceivable_and_inReality : ∃ (x : Being), Conceivable x ∧
-InReality x` (Step 3)
+* `lt_of_inUnderstanding_not_inReality_inReality {x y : Being} : InUnderstanding x → ¬InReality x →
+  InReality y → x < y` (Step 2)
+* `exists_conceivable_and_inReality : ∃ (x : Being), Conceivable x ∧ InReality x` (Step 3)
 * `IsGod.inUnderstanding {x : Being} : IsGod x → InUnderstanding x` (Step 8)
 
-Step 3 of the original formulation by Alvin Plantinga is the following
-premise: "A being having all of God’s properties plus existence in
-reality can be conceived." This premise is redundant. Since God is the
-greatest being that can be conceived, God itself can be conceived.
-Therefore, a being having all of God's properties can be conceived.
+Step 3 of the original formulation by Alvin Plantinga is the following premise: "A being having all
+of God’s properties plus existence in reality can be conceived." This premise is redundant. Since
+God is the greatest being that can be conceived, God itself can be conceived.  Therefore, a being
+having all of God's properties can be conceived.
 
-I think the conclusion of St. Anselm's argument is the following
-statement:
+I think the conclusion of St. Anselm's argument is the following statement:
 
 ```lean
 theorem IsGod.inReality {x : Being} : IsGod x → InReality x
 ```
 
-This theorem doesn't state that God exists in reality. It merely says
-that if a being is God, it exists in reality. In order to prove the
-existence of God in reality, you need to show that `∃ (x : Being), IsGod
-x ∧ InReality x`.
+This theorem doesn't state that God exists in reality. It merely says that if a being is God, it
+exists in reality. In order to prove the existence of God in reality, you need to show that `∃ (x :
+Being), IsGod x ∧ InReality x`.
 
-For this reason, I think St. Anselm's argument doesn't show God's
-existence. Of course, I might have formalized it wrong.
+For this reason, I think St. Anselm's argument doesn't show God's existence. Of course, I might have
+formalized it wrong.
 
 ## Theorem `not_exists_int_isGod`
 
-A user named car_nap of Owl of Sogang, a Korean-speaking philosophy
-discussion forum, [pointed out][owl] (in Korean) that I didn't prove
-that the statement `∃ (x : Being), IsGod x ∧ InReality x` is not a
-theorem of a theory whose axioms are the premises of St. Anselm's
-argument (and the axioms of Lean's type theory).
+A user named car_nap of Owl of Sogang, a Korean-speaking philosophy discussion forum, [pointed
+out][owl] (in Korean) that I didn't prove that the statement `∃ (x : Being), IsGod x ∧ InReality x`
+is not a theorem of a theory whose axioms are the premises of St. Anselm's argument (and the axioms
+of Lean's type theory).
 
-So I proved a theorem named `not_exists_int_isGod`, which shows that
-there exist a universe level `u`, a type `Being : Type u`, and an
-instance of `Anselm Being` where the statement `∃ (x : Being), IsGod x`
-is false.
+So I proved a theorem named `not_exists_int_isGod`, which shows that there exist a universe level
+`u`, a type `Being : Type u`, and an instance of `Anselm Being` where the statement `∃ (x : Being),
+IsGod x` is false.
 
 ## Reference
 
-* Oppy, Graham, "Ontological Arguments", *The Stanford Encyclopedia of
-Philosophy* (Fall 2023 Edition), Edward N. Zalta & Uri Nodelman (eds.),
-URL =
+* Oppy, Graham, "Ontological Arguments", *The Stanford Encyclopedia of Philosophy* (Fall 2023
+Edition), Edward N. Zalta & Uri Nodelman (eds.), URL =
 https://plato.stanford.edu/archives/fall2023/entries/ontological-arguments/.
 
 ## Acknowledgements
 
 ### The Lean community
 
-I'd like to thank Eric Wieser and Alistair Tucker. Eric Wieser found
-inconsistency in my first and second drafts. Alistair Tucker commented
-on transcribing premise 3 of the original formulation by Alvin
-Plantinga. You can see my discussion with them in [this
-link][leanzulip].
+I'd like to thank Eric Wieser and Alistair Tucker. Eric Wieser found inconsistency in my first and
+second drafts. Alistair Tucker commented on transcribing premise 3 of the original formulation by
+Alvin Plantinga. You can see my discussion with them in [this link][leanzulip].
 
-Alistair Tucker also [told me][tucker] how to prove that we can't deduce
-the statement `∃ (x : Being), IsGod x ∧ InReality x` from the premises
-of St. Anselm's argument and the axioms of Lean's type theory.
+Alistair Tucker also [told me][tucker] how to prove that we can't deduce the statement `∃ (x :
+Being), IsGod x ∧ InReality x` from the premises of St. Anselm's argument and the axioms of Lean's
+type theory.
 
 ### Owl of Sogang
 
@@ -102,11 +84,14 @@ I want to thank car_nap for raising [the issue mentioned
 above](#theorem-anselmnot_exists_int_isgod).
 
 [anselm]: ../../Notes/Anselm.lean
-[fst]: https://github.com/forked-from-1kasper/ground_zero/blob/9f83f7c6224eee8905b16aeebc4c234b4b216031/GroundZero/Theorems/Ontological.lean#L520-L521
+[fst]:
+https://github.com/forked-from-1kasper/ground_zero/blob/9f83f7c6224eee8905b16aeebc4c234b4b216031/GroundZero/Theorems/Ontological.lean#L520-L521
 [plantinga]: https://plato.stanford.edu/entries/ontological-arguments/#StAnsOntArg
 [owl]: https://forum.owlofsogang.com/t/lean/3613/9
-[leanzulip]: https://leanprover.zulipchat.com/#narrow/stream/113488-general/topic/Formalizing.20St.2E.20Anselm's.20ontological.20argument/near/39867934
-[tucker]: https://leanprover.zulipchat.com/#narrow/stream/116395-maths/topic/how.20do.20I.20say.20.22a.20sentence.20is.20a.20theorem.20of.20a.20theory.22.20in.20lean.3F/near/399042805
+[leanzulip]:
+https://leanprover.zulipchat.com/#narrow/stream/113488-general/topic/Formalizing.20St.2E.20Anselm's.20ontological.20argument/near/39867934
+[tucker]:
+https://leanprover.zulipchat.com/#narrow/stream/116395-maths/topic/how.20do.20I.20say.20.22a.20sentence.20is.20a.20theorem.20of.20a.20theory.22.20in.20lean.3F/near/399042805
 -/
 
 section PartialOrder
